\documentclass[12pt]{article}
\setlength{\oddsidemargin}{0in}
\setlength{\evensidemargin}{0in}
\setlength{\textwidth}{6.5in}
\setlength{\parindent}{0in}
\setlength{\parskip}{\baselineskip}

\usepackage{amsmath,amsfonts,amssymb}


\begin{document}

CS 527 Winter 2021 \hfill Homework 1\\
Hoang Vu-Kingston

\hrulefill

\begin{enumerate}

	\item\textit{Problem 1}\\
    Case 0 $\rightarrow$ 00000, 1 $\rightarrow$ 11111 and p=0.1\\
    Since majority voting is use for decoding, the probability of error is:
    \begin{align*}
        P_e  &= P_{\text{3/5 bits is wrong}} + P_{\text{4/5 bits is wrong}} + P_{\text{5/5 bits is wrong}} \\
        &= {5 \choose 3}p^3(1-p)^2 + {5 \choose 4}p^4(1-p) + {5 \choose 5}p^5\\
        &= 10 \times 0.1^3 \times 0.9^2 + 5 \times 0.1^4 \times 0.9 + 0.1^5\\
        &= 0.00856...
    \end{align*}

    Case 0 $\rightarrow$ 0000000, 1 $\rightarrow$ 1111111 and p=0.1\\
    Similarly:
    \begin{align*}
        P_e  &= P_{\text{4/7 bits is wrong}} + P_{\text{5/7 bits is wrong}} + P_{\text{6/7 bits is wrong}} + P_{\text{7/7 bits is wrong}}\\
        &= {7 \choose 4}p^4(1-p)^3 + {7 \choose 5}p^5(1-p)^2 + {7 \choose 6}p^6(1-p) + {7 \choose 7}p^7\\
        &= 35 \times 0.1^4 \times 0.9^3 + 21 \times 0.1^5 \times 0.9^2 + 7 \times 0.1^6 \times 0.9 + 0.1^7\\
        &= 0.002728...
    \end{align*}

    \item\textit{Problem 2}\\
    Possible outputs and their probabilities:
    \begin{align*}
        P(X_1) &= 1/8\\
        P(X_2) & = 1/7\\
        P(X_3) & = 1/6\\
        ...
    \end{align*}
    Thus:
    \begin{equation*}
        H(X) = (1/8*log_2(8)) + (1/7*log_2(7)) + ... + (1*log_2(1)) = 3.19958...
    \end{equation*}

    \item\textit{Problem 3}\\
    Possible outputs and their probabilities:
    \begin{align*}
        P(X_0) &= {47 \choose 5} / {50 \choose 5} \\
        P(X_1) &= {47 \choose 4} {3 \choose 1} / {50 \choose 5}\\
        P(X_2) &= {47 \choose 3} {3 \choose 2} / {50 \choose 5}\\
        P(X_3) &= {47 \choose 2} {3 \choose 3} / {50 \choose 5}\\
    \end{align*}
    Thus:
    \begin{align*}
        H(X) &= P(X_0)log_2(1/P(X_0)) + P(X_1)log_2(1/P(X_1))\\
             &+ P(X_2)log_2(1/P(X_2)) + P(X_3)log_2(1/P(X_3))\\
             &= 0.96935...
    \end{align*}

    \item\textit{Problem 4}\\
    Possible outputs for X and their probabilities:\\
    \begin{align*}
        &\text{A or B win in 4 games:}\\
        &P(X_1) = 2 \times {4 \choose 4}(0.5)^4(1-0.5)^0 = 0.125\\
        &\text{A or B win in 5 games: (win 3 games in set of 4 then win last game)}\\
        &P(X_1) = 2 \times {4 \choose 3}(0.5)^3(1-0.5)^1 \times 0.5 = 0.25\\
        &\text{A or B win in 6 games: (win 3 games in set of 5 then win last game)}\\
        &P(X_1) = 2 \times {5 \choose 3}(0.5)^3(1-0.5)^2 \times 0.5 = 0.3125\\
        &\text{A or B win in 4 games: (win 3 games in set of 6 then win last game}\\
        &P(X_1) = 2 \times {6 \choose 3}(0.5)^3(1-0.5)^3 \times 0.5 = 0.3125\\
    \end{align*}
    Thus:
    \begin{equation*}
        H(X) = 1.92379
    \end{equation*}

    The possible outputs and probabilities for Y are: \\
    \begin{align*}
        P(Y_1) &= \text{No. of possible 4 games conclusion} / \text{No. of games possible}\\
        &= 2{4 \choose 4} / 2 {7 \choose 4} = \frac{1}{35}\\
        \\
        P(Y_2) &= {4 \choose 3} / {7 \choose 4} = \frac{4}{35}\\
        \\
        P(Y_3) &= {5 \choose 3} / {7 \choose 4} = \frac{2}{7}\\
        \\
        P(Y_2) &= {6 \choose 3} / {7 \choose 4} = \frac{4}{7}\\
        \\
    \end{align*}
    Thus:
    \begin{equation*}
        H(Y) = 1.48192...
    \end{equation*}

    \item\textit{Problem 5}\\
    $P(X=0) = 2/3,  P(X = 1) = 1/3, p = 1/4$\\
    $\Rightarrow P(Y=0) = P(X=0)(1-p) = 1/2$\\
    $\Rightarrow P(Y=1) = P(X=1)(1-p) = 1/4$\\
    \begin{enumerate}
        \item $H(X), H(Y)$
        \begin{align*}
            H(X) &= P(X=0)log_2(1/P(X=0)) + P(X=1)log_2(1/P(X=1))\\
            \\
            &= \frac{2}{3}log_2(\frac{3}{2}) + \frac{1}{3}log_2(3)\\
            \\
            &= \frac{2}{3}(log_23 - 1) + \frac{1}{3}log_2(3)\\
            \\
            &= log_23 - \frac{2}{3}
        \end{align*}
        \begin{align*}
            H(Y) &= P(Y=0)log_2(1/P(Y=0)) + P(Y=1)log_2(1/P(Y=1))\\
            \\
            &= \frac{1}{2}log_2(2) + \frac{1}{4}log_24\\
            \\
            &= \frac{1}{2} + \frac{1}{4}2\\
            \\
            &= 1
        \end{align*}
        \item $H(X|Y), H(Y|X)$
        \begin{flalign*}
            &H(X|Y) = P(Y=0)H(X|Y=0) + P(Y=1)H(X|Y=1)\\
            &P(Y=0)H(X|Y=0) = \frac{1}{2} \times (P(X = 0 | Y = 0)log_2(1/P(X=0 | Y=0))\\
                           &+ P(X = 1 | Y = 0)log_2(1/P(X=1 | Y=0)))\\
                           \\
                           &= \frac{1}{2} (-P(Y=0 | X=0)P(X=0)log_2(P(Y=0 | X=0)P(X=0))\\
                           \\
                           &- P(Y=0 | X=1)P(X=1)log_2(P(Y=0 | X=01P(X=1))\\
                           \\
                           &= \frac{1}{2} (-\frac{3}{4}\times\frac{2}{3}log_2(\frac{3}{4}\times\frac{2}{3}) + 0)\\
                           \\
                           &= \frac{1}{4}\\
                           \\
            &P(Y=1)H(X|Y=1) = \frac{1}{4} \times (P(X = 0 | Y = 1)log_2(1/P(X=0 | Y=1))\\
                           \\
                           &+ P(X = 1 | Y = 1)log_2(1/P(X=1 | Y=1)))\\
                           \\
                           &= \frac{1}{4} (0 - P(Y=1|X=1)P(X=1)log_2(P(Y=1|X=1)P(X=1))\\
                           \\
                           &= \frac{1}{4} (0 - \frac{3}{4}\times\frac{1}{3}log_2(\frac{3}{4}\times\frac{1}{3}))\\
                           \\
                           &= \frac{1}{8}\\
            &H(X|Y) = \frac{1}{4} + \frac{1}{8} = \frac{3}{8}
        \end{flalign*}
        \begin{flalign*}
            &H(Y|X) = P(X=0)H(Y|X=0) + P(X=1)H(Y|X=1)\\
            &P(X=0)H(Y|X=0) = \frac{2}{3} \times (P(Y=0|X=0)log_2(1/P(Y=0|X=0))\\
                           &+ P(Y=1|X=0)log_2(1/P(Y=1 |X=0)))\\
                           \\
                           &= \frac{2}{3} (\frac{3}{4}log_2(\frac{4}{3}) + 0)\\
                           \\
                           &= \frac{1}{2}log_2(\frac{4}{3})\\
                           \\
            &P(X=1)H(Y|X=1) = \frac{1}{3} \times (P(Y=0|X=1)log_2(1/P(Y=0|X=1))\\
                           \\
                           &+ P(Y=1|X=1)log_2(1/P(Y=1|X=1)))\\
                           \\
                           &= \frac{1}{3} (0 + \frac{3}{4}log_2(\frac{4}{3}))\\
                           \\
                           &= \frac{1}{4}log_2(\frac{4}{3})\\
                           \\
            &H(Y|X) = \frac{3}{4}log_2(\frac{4}{3})\\
            \\
            &= \frac{3}{4}(log_24 - log_23) = \frac{3}{4}(2-log_23)
        \end{flalign*}
        \item $H(X,Y)$
        \begin{align*}
            H(X,Y) = H(X|Y) + H(Y) = \frac{3}{8} + 1 = \frac{11}{8}
        \end{align*}
        \item $I(X,Y)$
        \begin{align*}
            I(X,Y) = H(X) - H(X/Y) = log_23 - \frac{2}{3} - \frac{3}{8}
        \end{align*}
    \end{enumerate}
    \item\textit{Problem 6}\\
    Possible outputs and their probabilities: \\
    \begin{align*}
        P(X_1) &= \text{head in one flip} = 0.5\\
        P(X_2) &= 0.5^2\\
        P(X_3) &= 0.5^3\\
        P(X_4) &= 0.5^4\\
        ...\\
        P(X_n) &= 0.5^n\\
    \end{align*}
    Thus:
    \begin{align*}
        H(X) &= P(X_1)log_2(\frac{1}{P(X_1)}) + P(X_2)log_2(\frac{1}{P(X_2)}) + ... + P(X_n)log_2(\frac{1}{P(X_n)})\\
        &= \frac{1}{2}log_2(2) + \frac{1}{4}log_24 + ... + \frac{1}{2^n}log_2(2^n)\\
        &= \frac{1}{2} + \frac{2}{2^2} + \frac{3}{2^3} + ... + \frac{n}{2^n}\\
        \Rightarrow 2H(X) &=  \frac{2}{2} + \frac{2}{2^1} + \frac{3}{2^2} + ... + \frac{n}{2^n-1}\\
        \Rightarrow 2H(X) - H(X) &= 1 + (\frac{2}{2^1} - \frac{1}{2}) + (\frac{3}{2^2} - \frac{2}{2^2}) + ...\\
        \Rightarrow H(X) &=  1 + \frac{1}{2} + \frac{1}{4} + ... = 1 + 1 = 2
    \end{align*}
\newpage


\end{enumerate}

\end{document}
